src/lowparse/steel_st_array/LowParse.SteelST.Combinators.fst
@@ -1,0 +1,43 @@
+module LowParse.SteelST.Combinators
+include LowParse.Spec.Combinators
+include LowParse.SteelST.Validate
+include LowParse.SteelST.Access
+open Steel.ST.Util
+
+module AP = LowParse.SteelST.ArrayPtr
+module R = Steel.ST.Reference
+module SZ = LowParse.Steel.StdInt
+
+#set-options "--ide_id_info_off"
+
+module T = FStar.Tactics
+
+#push-options "--z3rlimit 24"
+#restart-solver
+
+let validate_pair
+  #k1 #t1 (#p1: parser k1 t1) (v1: validator p1)
+  #k2 #t2 (#p2: parser k2 t2) (v2: validator p2)
+: Tot (validator (p1 `nondep_then` p2))
+=
+  fun #_ #va a len err ->
+    nondep_then_eq p1 p2 (AP.contents_of' va);
+    let s1 = v1 a len err in
+    let _ = gen_elim () in
+    let verr = R.read err in
+    if verr = 0ul
+    then begin
+      let ar = AP.split a s1 in
+      let _ = gen_elim () in
+      let len2 = len `SZ.size_sub` s1 in
+      let s2 = v2 ar (len `SZ.size_sub` s1) err in
+      let _ = gen_elim () in
+      let _ = AP.join a ar in
+      noop ();
+      return (s1 `SZ.size_add` s2)
+    end
+    else
+    begin
+      noop ();
+      return s1
+    end
